src/Semantics.v
@@ -339,21 +339,57 @@ Ltac solve_type_of_extension r ty :=
   eenough (Rcd.type_of r = ty);
   [ solve_type_of | auto ].
 
+Module MatchMode.
+  Inductive t :=
+  | Explicit
+  | Full
+  .
+End MatchMode.
+Import MatchMode.
+
 Module PatternT.
   Definition T := Rcd.T.
 
-  Fixpoint type_of (pi : Pattern.t) : T :=
-    match pi with
-    | Pattern.start pv =>
-        (Pattern.vname pv |-> Value.GVertexT)
-    | Pattern.hop pi pe pv =>
-        (Pattern.vname pv |-> Value.GVertexT; Pattern.ename pe |-> Value.GEdgeT; type_of pi)
-    end.
+  Section type_of.
+    Fixpoint type_of_full (pi : Pattern.t) : T :=
+      match pi with
+      | Pattern.start pv =>
+          (Pattern.vname pv |-> Value.GVertexT)
+      | Pattern.hop pi pe pv =>
+          (Pattern.vname pv |-> Value.GVertexT; Pattern.ename pe |-> Value.GEdgeT; type_of_full pi)
+      end.
+
+    Fixpoint type_of_explicit (pi : Pattern.t) : T :=
+      match pi with
+      | Pattern.start pv =>
+        match Pattern.vname pv with
+        | Name.explicit _ => (Pattern.vname pv |-> Value.GVertexT)
+        | Name.implicit _ => Rcd.emptyT
+        end
+      | Pattern.hop pi pe pv =>
+        match Pattern.vname pv, Pattern.ename pe with
+        | Name.explicit _, Name.explicit _ =>
+          (Pattern.vname pv |-> Value.GVertexT; Pattern.ename pe |-> Value.GEdgeT; type_of_explicit pi)
+        | Name.explicit _, Name.implicit _ =>
+          (Pattern.vname pv |-> Value.GVertexT; type_of_explicit pi)
+        | Name.implicit _, Name.explicit _ =>
+          (Pattern.ename pe |-> Value.GEdgeT; type_of_explicit pi)
+        | Name.implicit _, Name.implicit _ =>
+          type_of_explicit pi
+        end
+      end.
+
+    Definition type_of (mode : MatchMode.t) (pi : Pattern.t) : T :=
+      match mode with
+      | Full => type_of_full pi
+      | Explicit => type_of_explicit pi
+      end.
+  End type_of.
 
   Lemma type_of__dom_vertices (pi : Pattern.t) nv
     (Hwf : Pattern.wf pi)
     (HIn : In nv (Pattern.dom_vertices pi)) :
-      type_of pi nv = Some Value.GVertexT.
+      type_of Full pi nv = Some Value.GVertexT.
   Proof.
     induction pi; simpls.
     all: desf.
@@ -367,7 +403,7 @@ Module PatternT.
   Lemma type_of__dom_edges (pi : Pattern.t) ne
     (Hwf : Pattern.wf pi)
     (HIn : In ne (Pattern.dom_edges pi)) :
-      type_of pi ne = Some Value.GEdgeT.
+      type_of Full pi ne = Some Value.GEdgeT.
   Proof.
     induction pi; simpls.
     all: desf.
@@ -383,7 +419,7 @@ Module PatternT.
 
   Lemma dom_vertices__type_of (pi : Pattern.t) nv
     (Hwf : Pattern.wf pi)
-    (Htype : type_of pi nv = Some Value.GVertexT) :
+    (Htype : type_of Full pi nv = Some Value.GVertexT) :
       In nv (Pattern.dom_vertices pi).
   Proof.
     induction pi; simpls.
@@ -393,7 +429,7 @@ Module PatternT.
 
   Lemma dom_edges__type_of (pi : Pattern.t) ne
     (Hwf : Pattern.wf pi)
-    (Htype : type_of pi ne = Some Value.GEdgeT) :
+    (Htype : type_of Full pi ne = Some Value.GEdgeT) :
       In ne (Pattern.dom_edges pi).
   Proof.
     induction pi; simpls.
@@ -403,44 +439,45 @@ Module PatternT.
 
   Theorem In_dom_vertices__iff (pi : Pattern.t) nv
     (Hwf : Pattern.wf pi) :
-      In nv (Pattern.dom_vertices pi) <-> type_of pi nv = Some Value.GVertexT.
+      In nv (Pattern.dom_vertices pi) <-> type_of Full pi nv = Some Value.GVertexT.
   Proof.
     split; eauto using type_of__dom_vertices, dom_vertices__type_of.
   Qed.
 
   Theorem In_dom_edges__iff (pi : Pattern.t) ne
     (Hwf : Pattern.wf pi) :
-      In ne (Pattern.dom_edges pi) <-> type_of pi ne = Some Value.GEdgeT.
+      In ne (Pattern.dom_edges pi) <-> type_of Full pi ne = Some Value.GEdgeT.
   Proof.
     split; eauto using type_of__dom_edges, dom_edges__type_of.
   Qed.
 
-  Theorem type_of__types (pi : Pattern.t) k :
-      type_of pi k = Some Value.GVertexT \/
-      type_of pi k = Some Value.GEdgeT \/
-      type_of pi k = None.
+  Theorem type_of__types mode pi k :
+      type_of mode pi k = Some Value.GVertexT \/
+      type_of mode pi k = Some Value.GEdgeT \/
+      type_of mode pi k = None.
   Proof.
     induction pi; simpls.
+    all: destruct mode; simpls.
     all: desf_unfold_pat.
-    all: eauto with pattern_wf_db.
   Qed.
 
   Theorem In_dom__iff (pi : Pattern.t) k
     (Hwf : Pattern.wf pi) :
-      In k (Pattern.dom pi) <-> PartialMap.in_dom k (type_of pi).
+      In k (Pattern.dom pi) <-> PartialMap.in_dom k (type_of Full pi).
   Proof.
     rewrite Pattern.In_dom.
     rewrite In_dom_vertices__iff, In_dom_edges__iff; auto.
     unfold PartialMap.in_dom.
     split; ins.
     all: desf; eauto.
-    edestruct type_of__types as [? | [? | ?]]; eauto.
+    edestruct type_of__types with (mode := Full) as [? | [? | ?]].
+    all: simpls; eauto.
     congruence.
   Qed.
 
   Corollary not_In_dom__iff (pi : Pattern.t) k
     (Hwf : Pattern.wf pi) :
-      ~ (In k (Pattern.dom pi)) <-> type_of pi k = None.
+      ~ (In k (Pattern.dom pi)) <-> type_of Full pi k = None.
   Proof.
     rewrite In_dom__iff; auto.
     now rewrite PartialMap.not_in_dom_iff.
@@ -448,7 +485,7 @@ Module PatternT.
 
   Corollary matches_pattern_dom__if (pi : Pattern.t) r
     (Hwf : Pattern.wf pi)
-    (Htype : Rcd.type_of r = type_of pi) :
+    (Htype : Rcd.type_of r = type_of Full pi) :
       Rcd.matches_pattern_dom r pi.
   Proof.
     unfold Rcd.matches_pattern_dom; ins.
@@ -458,7 +495,7 @@ Module PatternT.
 
   Lemma wf__type_of_pe pi pe pv
     (Hwf : Pattern.wf (Pattern.hop pi pe pv)) :
-      type_of pi (Pattern.ename pe) = None.
+      type_of Full pi (Pattern.ename pe) = None.
   Proof.
     rewrite <- not_In_dom__iff. 
     all: eauto with pattern_wf_db.
@@ -467,7 +504,7 @@ Module PatternT.
   Lemma wf__type_of_pv__None pi pe pv
     (Hwf : Pattern.wf (Pattern.hop pi pe pv))
     (HIn : ~ In (Pattern.vname pv) (Pattern.dom_vertices pi)) :
-      type_of pi (Pattern.vname pv) = None.
+      type_of Full pi (Pattern.vname pv) = None.
   Proof.
     rewrite <- not_In_dom__iff. 
     all: eauto with pattern_wf_db.
@@ -476,7 +513,7 @@ Module PatternT.
   Lemma wf__type_of_pv__Some pi pe pv
     (Hwf : Pattern.wf (Pattern.hop pi pe pv))
     (HIn : In (Pattern.vname pv) (Pattern.dom_vertices pi)) :
-      type_of pi (Pattern.vname pv) = Some Value.GVertexT.
+      type_of Full pi (Pattern.vname pv) = Some Value.GVertexT.
   Proof.
     rewrite <- In_dom_vertices__iff. 
     all: eauto with pattern_wf_db.
@@ -488,7 +525,6 @@ Module PatternT.
 End PatternT.
 
 Module Path.
-
   Inductive t :=
   | start (v : vertex)
   | hop (p : t) (e : edge) (v : vertex).
@@ -502,20 +538,36 @@ Module Path.
   Section matches.
     Import Pattern.
 
+    Variable mode : MatchMode.t.
     Variable g : PropertyGraph.t.
     Variable r : Rcd.t.
 
-    Record matches_pvertex (v : vertex) (p : pvertex) : Prop := {
+    Definition matches_name_full (n : Name.t) (v : Value.t) : Prop := 
+      r n = Some v.
+
+    Definition matches_name_explicit (n : Name.t) (v : Value.t) : Prop := 
+      match n with
+      | Name.implicit _ => True
+      | Name.explicit _ => r n = Some v
+      end.
+
+    Definition matches_name (n : Name.t) (v : Value.t) : Prop := 
+      match mode with
+      | Full => matches_name_full n v
+      | Explicit => matches_name_explicit n v
+      end.
+
+    Record matches_pvertex (v : vertex) (pv : pvertex) : Prop := {
         vertex_in_g : In v (PropertyGraph.vertices g);
-        matches_vname : r (Pattern.vname p) = Some (Value.GVertex v);
-        matches_vlabel : forall l, Pattern.vlabel p = Some l ->
+        matches_vname : matches_name (Pattern.vname pv) (Value.GVertex v);
+        matches_vlabel : forall l, Pattern.vlabel pv = Some l ->
           In l (PropertyGraph.vlabels g v);
       }.
 
-    Record matches_pedge (e : edge) (p : pedge) : Prop := {
+    Record matches_pedge (e : edge) (pe : pedge) : Prop := {
         edge_in_g : In e (PropertyGraph.edges g);
-        matches_ename : r (Pattern.ename p) = Some (Value.GEdge e);
-        matches_elabel : forall l, Pattern.elabel p = Some l ->
+        matches_ename : matches_name (Pattern.ename pe) (Value.GEdge e);
+        matches_elabel : forall l, Pattern.elabel pe = Some l ->
           PropertyGraph.elabel g e = l;
       }.
 
@@ -566,53 +618,122 @@ Module Path.
     .
   End matches.
 
-  Lemma matches_in_dom graph path pi r' n
-    (Hmatch : matches graph r' path pi)
+  #[global]
+  Hint Unfold matches_name_full matches_name_explicit matches_name : matches_name_db.
+
+  Theorem matches_name__full_explicit r n v
+    (Hmatch : matches_name Full r n v) :
+      matches_name Explicit r n v.
+  Proof.
+    autounfold with matches_name_db.
+    destruct n; auto.
+  Qed.
+
+  Theorem matches_pvertex__full_explicit graph r v pv
+    (Hmatch : matches_pvertex Full graph r v pv) :
+      matches_pvertex Explicit graph r v pv.
+  Proof.
+    destruct Hmatch; constructor; auto.
+    now apply matches_name__full_explicit.
+  Qed.
+
+  Theorem matches_pedge__full_explicit graph r e pe
+    (Hmatch : matches_pedge Full graph r e pe) :
+      matches_pedge Explicit graph r e pe.
+  Proof.
+    destruct Hmatch; constructor; auto.
+    now apply matches_name__full_explicit.
+  Qed.
+
+  Theorem matches__full_explicit graph path pi r
+    (Hmatch : matches Full graph r path pi) :
+      matches Explicit graph r path pi.
+  Proof.
+    induction Hmatch.
+    all: constructor; auto.
+    all: try now apply matches_pvertex__full_explicit.
+    all: try now apply matches_pedge__full_explicit.
+  Qed.
+
+  Theorem matches_full_in_dom graph path pi r' n
+    (Hmatch : matches Full graph r' path pi)
     (HIn : In n (Pattern.dom pi)) :
       PartialMap.in_dom n r'.
   Proof.
     unfold PartialMap.in_dom.
     induction Hmatch.
     all: destruct Hpv; try destruct Hpe.
+    all: unfold matches_name in *.
     all: simpls; desf.
     all: eauto.
   Qed.
 
-  Lemma matches_in_dom_contra graph path pi r' n
-    (Hmatch : matches graph r' path pi)
+  Theorem matches_explicit_in_dom graph path pi r' n
+    (Hmatch : matches Explicit graph r' path pi)
+    (HIn : In (Name.explicit n) (Pattern.dom pi)) :
+      PartialMap.in_dom (Name.explicit n) r'.
+  Proof.
+    unfold PartialMap.in_dom.
+    induction Hmatch.
+    all: destruct Hpv; try destruct Hpe.
+    all: autounfold with matches_name_db in *.
+    all: simpls; desf.
+    all: eauto.
+  Qed.
+
+  Theorem matches_full_in_dom_contra graph path pi r' n
+    (Hmatch : matches Full graph r' path pi)
     (Hval : r' n = None) :
       ~ In n (Pattern.dom pi).
   Proof.
     intro contra.
-    eapply matches_in_dom in contra; eauto.
+    eapply matches_full_in_dom in contra; eauto.
     unfold PartialMap.in_dom in contra.
     desf.
   Qed.
 
-  Lemma matches_last graph path pi r'
-    (Hmatch : matches graph r' path pi) :
+  Theorem matches_explicit_in_dom_contra graph path pi r' n
+    (Hmatch : matches Explicit graph r' path pi)
+    (Hval : r' (Name.explicit n) = None) :
+      ~ In n (Pattern.dom_explicit pi).
+  Proof.
+    intro contra.
+    rewrite Pattern.In_dom_explicit in contra.
+    eapply matches_explicit_in_dom in contra; eauto.
+    unfold PartialMap.in_dom in contra.
+    desf.
+  Qed.
+
+  Theorem matches_full_last graph path pi r'
+    (Hmatch : matches Full graph r' path pi) :
       r' (Pattern.vname (Pattern.last pi)) = Some (Value.GVertex (Path.last path)).
   Proof.
     destruct pi. 
     all: inv Hmatch.
     all: destruct Hpv; try destruct Hpe.
+    all: simpls.
+    all: unfold matches_name in *; desf.
     all: eauto.
   Qed.
 
-  Lemma matches_exclude graph path pi r' n x
-    (Hmatch : matches graph r' path pi)
+  Theorem matches_exclude mode graph path pi r' n x
+    (Hmatch : matches mode graph r' path pi)
     (HIn : ~ In n (Pattern.dom pi)) :
-      matches graph (n !-> x; r') path pi.
+      matches mode graph (n !-> x; r') path pi.
   Proof.
-    induction Hmatch.
+    destruct mode.
+    all: induction Hmatch.
     all: destruct Hpv; try destruct Hpe.
-    1: apply matches_nil.
-    2: apply matches_cons.
+    all: try apply matches_nil.
+    all: try apply matches_cons.
+    all: unfold matches_name in *; desf.
     all: try apply IHHmatch.
     all: try (intro; apply HIn; right; now right).
     all: try apply Path.Build_matches_pvertex.
     all: try apply Path.Build_matches_pedge.
     all: auto.
+    all: autounfold with matches_name_db in *.
+    all: desf; ins.
     all: desf_unfold_pat.
     all: exfalso; auto.
   Qed.
@@ -848,20 +969,19 @@ Module EvalQuery.
       PropertyGraph.wf graph -> Pattern.wf pattern ->
         exists table', eval_match_clause graph pattern = Some table'.
 
-    Axiom match_clause_type : forall graph pattern table' r',
+    Axiom match_clause_type : forall graph pattern table',
       eval_match_clause graph pattern = Some table' ->
-        Pattern.wf pattern -> In r' table' ->
-          Rcd.type_of r' = PatternT.type_of pattern.
+        Pattern.wf pattern ->
+          BindingTable.of_type table' (PatternT.type_of Full pattern).
 
     Axiom match_clause_spec : forall graph path pattern table' r',
       eval_match_clause graph pattern = Some table' ->
-        Pattern.wf pattern -> Rcd.type_of r' = PatternT.type_of pattern ->
-          Path.matches graph r' path pattern -> In r' table'.
+        Pattern.wf pattern -> Rcd.type_of r' = PatternT.type_of Full pattern ->
+          Path.matches Full graph r' path pattern -> In r' table'.
 
     Axiom match_clause_spec' : forall graph pattern table' r',
       eval_match_clause graph pattern = Some table' ->
         PropertyGraph.wf graph -> Pattern.wf pattern -> In r' table' ->
-          exists path, Path.matches graph r' path pattern /\
-            Rcd.type_of r' = PatternT.type_of pattern.
+          exists path, Path.matches Full graph r' path pattern.
   End Spec.
 End EvalQuery.
