src/Translation.v
@@ -21,6 +21,7 @@ Import PropertyGraph.
 Import ExecutionPlan.
 Import FilterMode.
 Import ExpandMode.
+Import MatchMode.
 
 Section translate_pattern.
   Import Pattern.
@@ -57,14 +58,14 @@ Ltac desf_translate_pvertex_pedge :=
   desf; simpls;
   normalize_bool.
 
-Lemma type_of__rcd__pattern__cases pi r :
-  Rcd.type_of r = PatternT.type_of pi <->
+Lemma type_of__rcd__pattern__cases mode pi r :
+  Rcd.type_of r = PatternT.type_of mode pi <->
     (forall n, Rcd.type_of r n = Some Value.GVertexT <->
-      PatternT.type_of pi n = Some Value.GVertexT) /\
+      PatternT.type_of mode pi n = Some Value.GVertexT) /\
     (forall n, Rcd.type_of r n = Some Value.GEdgeT <->
-      PatternT.type_of pi n = Some Value.GEdgeT) /\
+      PatternT.type_of mode pi n = Some Value.GEdgeT) /\
     (forall n, Rcd.type_of r n = None <->
-      PatternT.type_of pi n = None).
+      PatternT.type_of mode pi n = None).
 Proof.
   split.
   { intros Heq; rewrite Heq.
@@ -79,7 +80,7 @@ Proof.
 Qed.
 
 Theorem type_of__translate_pattern pi (Hwf : Pattern.wf pi) :
-  type_of (translate_pattern pi) = PatternT.type_of pi.
+  type_of (translate_pattern pi) = PatternT.type_of Full pi.
 Proof.
   all: induction pi; simpls.
   all: desf_translate_pvertex_pedge.
@@ -124,19 +125,6 @@ Proof.
   all: congruence.
 Qed.
 
-Corollary translate_pattern__type_of_None_iff pi n (Hwf : Pattern.wf pi) :
-  ~ In n (Pattern.dom_vertices pi) /\ ~ In n (Pattern.dom_edges pi) <->
-    type_of (translate_pattern pi) n = None.
-Proof.
-  split.
-  { intros [? ?]. apply translate_pattern__type_of_None; assumption. }
-  ins. split.
-  all: intros contra.
-  1: apply translate_pattern__type_of_GVertexT in contra; try assumption.
-  2: apply translate_pattern__type_of_GEdgeT   in contra; try assumption.
-  all: congruence.
-Qed.
-
 Theorem translate_pattern_wf pi (Hwf : Pattern.wf pi) :
   ExecutionPlan.wf (translate_pattern pi).
 Proof.
@@ -145,13 +133,13 @@ Proof.
   all: unfold translate_pvertex, translate_pedge.
   all: desf; simpls; splits; auto.
   all: normalize_bool.
+  all: desf_unfold_pat.
   all: try apply translate_pattern__type_of_GVertexT; try assumption.
+  all: try apply translate_pattern__type_of_GEdgeT; try assumption.
   all: try apply translate_pattern__type_of_None; try assumption.
   all: eauto with pattern_wf_db.
 
-  all: desf_unfold_pat.
   all: try contradiction.
-  all: try apply translate_pattern__type_of_GVertexT; try assumption.
   all: try intro; exfalso.
   all: try (eapply Pattern.wf__pv_neq_pe; now eauto).
   all: try (eapply Pattern.wf__last_neq_pe; now eauto).
@@ -174,11 +162,14 @@ Module EvalQueryImpl (S : ExecutionPlan.Spec) : EvalQuery.Spec.
     now apply translate_pattern_wf.
   Qed.
 
-  Theorem match_clause_type_of graph pi table'
-    (Hres : eval_match_clause graph pi = Some table') :
-    BindingTable.of_type table' (type_of (translate_pattern pi)).
+  Theorem match_clause_type graph pi table'
+    (Hres : eval_match_clause graph pi = Some table')
+    (Hwf : Pattern.wf pi) :
+      BindingTable.of_type table' (PatternT.type_of Full pi).
   Proof.
-    eapply eval_type_of; eassumption.
+    unfold eval_match_clause in Hres.
+    apply eval_type_of in Hres.
+    rewrite type_of__translate_pattern in Hres; auto.
   Qed.
 
   Ltac desf_match_result Hres :=
@@ -194,19 +185,8 @@ Module EvalQueryImpl (S : ExecutionPlan.Spec) : EvalQuery.Spec.
     all: eauto.
   Qed.
 
-  Theorem match_clause_type graph pi table' r'
-    (Hres : eval_match_clause graph pi = Some table')
-    (Hwf : Pattern.wf pi)
-    (HIn : In r' table') :
-      Rcd.type_of r' = PatternT.type_of pi.
-  Proof.
-    unfold eval_match_clause in Hres.
-    apply eval_type_of in Hres.
-    rewrite type_of__translate_pattern in Hres; auto.
-  Qed.
-
   Lemma matches_pattern_type_start r' pv v
-    (Htype : Rcd.type_of r' = PatternT.type_of (Pattern.start pv))
+    (Htype : Rcd.type_of r' = PatternT.type_of Full (Pattern.start pv))
     (Hval : r' (Pattern.vname pv) = Some (Value.GVertex v)) :
       r' = (Pattern.vname pv |-> Value.GVertex v).
   Proof.
@@ -214,15 +194,6 @@ Module EvalQueryImpl (S : ExecutionPlan.Spec) : EvalQuery.Spec.
     apply (f_equal (fun f => f k)) in Htype.
     desf_unfold_pat.
     now apply Rcd.type_of_None.
-  Qed.
-
-  Lemma matches_pattern_type_start' r' pv v
-    (Hval : r' = (Pattern.vname pv |-> Value.GVertex v)) :
-      Rcd.type_of r' = PatternT.type_of (Pattern.start pv).
-  Proof.
-    extensionality k.
-    subst. simpl.
-    now rewrite Rcd.type_of_singleton.
   Qed.
 
   Definition expansion_of_by_hop' graph r' r mode v_from e v_to pi pe pv :=
@@ -235,10 +206,10 @@ Module EvalQueryImpl (S : ExecutionPlan.Spec) : EvalQuery.Spec.
 
   Lemma matches_pattern_type_exclude_All pi pe pv r'
     (Hwf : Pattern.wf (Pattern.hop pi pe pv))
-    (Htype : Rcd.type_of r' = PatternT.type_of (Pattern.hop pi pe pv))
+    (Htype : Rcd.type_of r' = PatternT.type_of Full (Pattern.hop pi pe pv))
     (HIn : ~ In (Pattern.vname pv) (Pattern.dom_vertices pi)) :
       Rcd.type_of (Pattern.ename pe !-> None; Pattern.vname pv !-> None; r') =
-        PatternT.type_of pi.
+        PatternT.type_of Full pi.
   Proof.
     assert (Hwf': Pattern.wf pi) by (eauto with pattern_wf_db).
     repeat rewrite Rcd.type_of_t_update; simpls.
@@ -251,9 +222,9 @@ Module EvalQueryImpl (S : ExecutionPlan.Spec) : EvalQuery.Spec.
 
   Lemma matches_pattern_type_exclude_Into pi pe pv r'
     (Hwf : Pattern.wf (Pattern.hop pi pe pv))
-    (Htype : Rcd.type_of r' = PatternT.type_of (Pattern.hop pi pe pv))
+    (Htype : Rcd.type_of r' = PatternT.type_of Full (Pattern.hop pi pe pv))
     (HIn : In (Pattern.vname pv) (Pattern.dom_vertices pi)) :
-      Rcd.type_of (Pattern.ename pe !-> None; r') = PatternT.type_of pi.
+      Rcd.type_of (Pattern.ename pe !-> None; r') = PatternT.type_of Full pi.
   Proof.
     assert (Hwf': Pattern.wf pi) by (eauto with pattern_wf_db).
     rewrite Rcd.type_of_t_update; simpls.
@@ -266,24 +237,25 @@ Module EvalQueryImpl (S : ExecutionPlan.Spec) : EvalQuery.Spec.
 
   Lemma matches_hop_All graph path e v pi pe pv r'
     (Hwf : Pattern.wf (Pattern.hop pi pe pv))
-    (Htype : Rcd.type_of r' = PatternT.type_of (Pattern.hop pi pe pv))
-    (Hmatch : Path.matches graph r' (Path.hop path e v) (Pattern.hop pi pe pv))
+    (Htype : Rcd.type_of r' = PatternT.type_of Full (Pattern.hop pi pe pv))
+    (Hmatch : Path.matches Full graph r' (Path.hop path e v) (Pattern.hop pi pe pv))
     (HIn : ~ In (Pattern.vname pv) (Pattern.dom_vertices pi)) :
       exists r, << Hexp : expansion_of_by_hop graph r' r All pi pe pv >> /\
-                << Hmatch' : Path.matches graph r path pi >> /\
-                << Htype' : Rcd.type_of r = PatternT.type_of pi >>.
+                << Hmatch' : Path.matches Full graph r path pi >> /\
+                << Htype' : Rcd.type_of r = PatternT.type_of Full pi >>.
   Proof.
     exists (Pattern.ename pe !-> None; Pattern.vname pv !-> None; r').
     inv Hmatch.
     destruct Hpe, Hpv.
+    autounfold with matches_name_db in *.
     splits.
     { unfold expansion_of_by_hop, expansion_of, expansion_of'.
       do 3 eexists. splits; eauto.
       all: try extensionality k.
       all: desf_unfold_pat.
+      all: try eauto using Path.matches_full_last.
       all: try (exfalso; eapply Pattern.wf__pe_neq_last; now eauto).
-      { exfalso. apply HIn. rewrite e0. apply Pattern.last__dom_vertices. }
-      eauto using Path.matches_last. }
+      exfalso; apply HIn. rewrite e0. apply Pattern.last__dom_vertices. }
     { apply Path.matches_exclude. apply Path.matches_exclude.
       all: eauto with pattern_wf_db. }
     { apply matches_pattern_type_exclude_All; eauto. }
@@ -291,16 +263,17 @@ Module EvalQueryImpl (S : ExecutionPlan.Spec) : EvalQuery.Spec.
 
   Lemma matches_hop_Into graph path e v pi pe pv r'
     (Hwf : Pattern.wf (Pattern.hop pi pe pv))
-    (Htype : Rcd.type_of r' = PatternT.type_of (Pattern.hop pi pe pv))
-    (Hmatch : Path.matches graph r' (Path.hop path e v) (Pattern.hop pi pe pv))
+    (Htype : Rcd.type_of r' = PatternT.type_of Full (Pattern.hop pi pe pv))
+    (Hmatch : Path.matches Full graph r' (Path.hop path e v) (Pattern.hop pi pe pv))
     (HIn : In (Pattern.vname pv) (Pattern.dom_vertices pi)) :
       exists r, << Hexp : expansion_of_by_hop graph r' r Into pi pe pv >> /\
-                << Hmatch' : Path.matches graph r path pi >> /\
-                << Hdom' : Rcd.type_of r = PatternT.type_of pi >>.
+                << Hmatch' : Path.matches Full graph r path pi >> /\
+                << Hdom' : Rcd.type_of r = PatternT.type_of Full pi >>.
   Proof.
     exists (Pattern.ename pe !-> None; r').
     inv Hmatch.
     destruct Hpe, Hpv.
+    autounfold with matches_name_db in *.
     eauto.
     splits.
     { unfold expansion_of_by_hop, expansion_of, expansion_of'.
@@ -310,7 +283,7 @@ Module EvalQueryImpl (S : ExecutionPlan.Spec) : EvalQuery.Spec.
       all: desf_unfold_pat.
       all: try (exfalso; eapply Pattern.wf__pe_neq_last; now eauto).
       all: try (exfalso; eapply Pattern.wf__pe_neq_pv; now eauto).
-      eauto using Path.matches_last. }
+      eauto using Path.matches_full_last. }
     { apply Path.matches_exclude.
       all: eauto with pattern_wf_db. }
     { eapply matches_pattern_type_exclude_Into; eauto. }
@@ -319,8 +292,8 @@ Module EvalQueryImpl (S : ExecutionPlan.Spec) : EvalQuery.Spec.
   Theorem match_clause_spec graph path pi table' r'
     (Hres : eval_match_clause graph pi = Some table')
     (Hwf : Pattern.wf pi)
-    (Htype : Rcd.type_of r' = PatternT.type_of pi)
-    (Hmatch : Path.matches graph r' path pi) :
+    (Htype : Rcd.type_of r' = PatternT.type_of Full pi)
+    (Hmatch : Path.matches Full graph r' path pi) :
       In r' table'.
   Proof.
     gen_dep Htype Hres r' table' path.
@@ -359,46 +332,28 @@ Module EvalQueryImpl (S : ExecutionPlan.Spec) : EvalQuery.Spec.
     all: eauto with pattern_wf_db.
   Qed.
 
-  Lemma matches_pattern_type_hop graph mode r r' pi pe pv
-    (Hwf : Pattern.wf (Pattern.hop pi pe pv))
-    (Htype : Rcd.type_of r = PatternT.type_of pi)
-    (Hexp : expansion_of_by_hop graph r' r mode pi pe pv) :
-      Rcd.type_of r' = PatternT.type_of (Pattern.hop pi pe pv).
-  Proof.
-    unfold expansion_of_by_hop, expansion_of, expansion_of' in Hexp.
-    unfold Rcd.matches_pattern_dom, PartialMap.in_dom in *.
-    ins; desf; desf.
-    all: repeat rewrite Rcd.type_of_update; simpls.
-    all: rewrite <- Htype.
-    { reflexivity. }
-
-    extensionality k.
-    desf_unfold_pat.
-    { exfalso; eapply Pattern.wf__pv_neq_pe; eauto. }
-    now rewrite Hval_to.
-  Qed.
-
   Lemma matches_expansion_of graph mode r r' path v_from e v_to pi pe pv
     (Hg_wf : PropertyGraph.wf graph)
     (Hwf : Pattern.wf (Pattern.hop pi pe pv))
-    (Hdom : Path.matches graph r path pi)
+    (Hdom : Path.matches Full graph r path pi)
     (Hvlabel : forall l : label, Pattern.vlabel pv = Some l -> In l (vlabels graph v_to))
     (Helabel : forall l : label, Pattern.elabel pe = Some l -> elabel graph e = l)
     (Hexp : expansion_of_by_hop' graph r' r mode v_from e v_to pi pe pv) :
-      Path.matches graph r' (Path.hop path e v_to) (Pattern.hop pi pe pv).
+      Path.matches Full graph r' (Path.hop path e v_to) (Pattern.hop pi pe pv).
   Proof.
     apply Path.matches_cons.
     all: unfold expansion_of_by_hop', expansion_of', expansion_of in Hexp.
     all: desf; desf.
     all: try apply Path.matches_exclude.
     all: try apply Path.matches_exclude.
-    all: eauto using Path.matches_in_dom_contra.
+    all: eauto using Path.matches_full_in_dom_contra.
     all: try apply Path.Build_matches_pedge.
     all: try apply Path.Build_matches_pvertex.
+    all: autounfold with matches_name_db in *.
     all: auto.
 
     all: assert (Path.last path = v_from)
-          by (erewrite Path.matches_last in Hval_from; eauto;
+          by (erewrite Path.matches_full_last in Hval_from; eauto;
             injection Hval_from; trivial).
     all: subst; auto.
 
@@ -415,8 +370,7 @@ Module EvalQueryImpl (S : ExecutionPlan.Spec) : EvalQuery.Spec.
     (Hg_wf : PropertyGraph.wf graph)
     (Hwf : Pattern.wf pi)
     (HIn : In r' table') :
-      exists path, Path.matches graph r' path pi /\
-        Rcd.type_of r' = PatternT.type_of pi.
+      exists path, Path.matches Full graph r' path pi.
   Proof.
     gen_dep Hres r' table'.
     induction pi; ins.
@@ -435,20 +389,19 @@ Module EvalQueryImpl (S : ExecutionPlan.Spec) : EvalQuery.Spec.
          | [H : expand _ _ _ _ _ _ _ = _ |- _ ] =>
             eapply expand_spec' in H; try eassumption; desf
          end.
-    all: try edestruct IHpi as [path [? ?]];
+    all: try edestruct IHpi as [path ?];
             eauto with pattern_wf_db.
+
     all: unfold expansion_of_by_hop, expansion_of in *; desf.
-    1-2: eexists (Path.start _); splits.
-    5-12: eexists (Path.hop path _ _); splits.
+    1-2: eexists (Path.start _).
+    all: try eexists (Path.hop path _ _).
+
+    all: try eapply Path.matches_nil, Path.Build_matches_pvertex.
+    all: autounfold with matches_name_db in *; eauto.
+    all: try now rewrite PartialMap.update_eq.
 
     all: try eapply matches_expansion_of; eauto.
-    all: try eapply matches_pattern_type_hop.
     all: try unfold expansion_of_by_hop, expansion_of.
-    all: eauto using matches_pattern_type_start'.
-
-    all: try eapply Path.matches_nil, Path.Build_matches_pvertex; eauto.
-    all: try rewrite PartialMap.update_eq.
-    all: auto.
 
     all: ins.
     all: try unfold expansion_of' in *; desf.
